Begin conversion to new RA for abstract history

src/high/resources/abstract_history.v
@@ -6,10 +6,10 @@ From iris.base_logic.lib Require Import own.
 From iris.heap_lang Require Export locations.
 From iris.proofmode Require Import proofmode.
 
-From self.algebra Require Import ghost_map.
+From self.algebra Require Import ghost_map ghost_map_map.
 From self.lang Require Import lang.
 From self Require Import extra.
-From self.high.resources Require Import auth_map_map.
+(* From self.high.resources Require Import auth_map_map. *)
 
 (* For abstract history we need two types of fragmental knowledge. One that
 represents ownership about the entire abstract history of a location (for
@@ -18,14 +18,15 @@ abstract history. *)
 
 (* Resource algebras that for each location stores the encoded abstract states
 associated with each message/store. *)
-Definition encoded_abs_historyR := gmapUR time (agreeR positiveO).
+(* Definition encoded_abs_historyR := gmapUR time (agreeR positiveO). *)
 
-Definition know_abs_historiesR := auth_map_mapR positiveO.
+(* Definition know_abs_historiesR := auth_map_mapR positiveO. *)
 
 (** We define a few things about the resource algebra that that we use to encode
 abstract histories. *)
 Section abs_history_lemmas.
-  Context `{!ghost_mapG Σ loc (gmap time positive), inG Σ know_abs_historiesR}.
+  Context `{ghost_map_mapG Σ loc time positive}.
+  (* Context `{!ghost_mapG Σ loc (gmap time positive), inG Σ know_abs_historiesR}. *)
   Context `{Countable ST}.
 
   Implicit Types
@@ -33,17 +34,19 @@ Section abs_history_lemmas.
     (enc_abs_hist : gmap time positive)
     (abs_hists : gmap loc (gmap time positive)).
 
-  Definition abs_hist_to_ra abs_hist : encoded_abs_historyR :=
-    (to_agree ∘ encode) <$> abs_hist.
+  (* Definition abs_hist_to_ra abs_hist : encoded_abs_historyR := *)
+  (*   (to_agree ∘ encode) <$> abs_hist. *)
 
   (* If we own the full history then we own the authorative view of both the
   resource algebras. *)
-  Definition own_full_history γ1 γ2 abs_hists : iProp Σ :=
-    ghost_map_auth γ1 (DfracOwn 1) abs_hists ∗
-    auth_map_map_auth γ2 abs_hists.
+  Definition history_full_map γ abs_hists : iProp Σ :=
+    full_map γ (DfracOwn 1) abs_hists.
 
-  Definition own_frag_encoded_history_loc γ2 ℓ enc_abs_hist : iProp Σ :=
-    auth_map_map_frag γ2 {[ ℓ := enc_abs_hist ]}.
+  Definition history_frag_entry γ ℓ t e : iProp Σ :=
+    frag_entry γ ℓ t e.
+
+  (* Definition history_frag_entry γ ℓ enc_abs_hist : iProp Σ := *)
+  (*   full_entry γ ℓ enc_abs_hist. *)
 
   (* In this definition we store that decoding the stored encoded histry is
   equal to our abstract history. This is weaker than strogin the other way
@@ -53,284 +56,260 @@ Section abs_history_lemmas.
   return [store_lb] for the returned state. At that point we can conclude that
   decoding the encoding gives a result but not that the encoding is an encoding
   of some state. *)
-  Definition own_frag_history_loc γ ℓ abs_hist : iProp Σ :=
-    ∃ enc,
-      ⌜decode <$> enc = Some <$> abs_hist⌝ ∗
-      own_frag_encoded_history_loc γ ℓ enc.
+  Definition history_frag_entry_unenc γ ℓ t (s : ST) : iProp Σ :=
+    ∃ e, ⌜ decode e = Some s ⌝ ∗ history_frag_entry γ ℓ t e.
 
-  Definition own_full_encoded_history_loc γ1 γ2 ℓ q enc_abs_hist : iProp Σ :=
-    ℓ ↪[ γ1 ]{#q} enc_abs_hist ∗
-    own_frag_encoded_history_loc γ2 ℓ enc_abs_hist.
+  Definition own_full_encoded_history_loc γ ℓ q enc_abs_hist : iProp Σ :=
+    full_entry γ ℓ (DfracOwn q) enc_abs_hist.
+    (* ℓ ↪[ γ ]{#q} enc_abs_hist ∗ *)
+    (* history_frag_entry ℓ enc_abs_hist. *)
 
-  Definition own_full_history_loc γ1 γ2 ℓ q abs_hist : iProp Σ :=
-    own_full_encoded_history_loc γ1 γ2 ℓ q (encode <$> abs_hist).
+  Definition history_full_map_loc γ ℓ q abs_hist : iProp Σ :=
+    own_full_encoded_history_loc γ ℓ q (encode <$> abs_hist).
 
-  Global Instance own_full_encoded_history_fractional γ1 γ2 ℓ enc_abs_hist :
-    Fractional (λ q, own_full_encoded_history_loc γ1 γ2 ℓ q enc_abs_hist).
-  Proof.
-    intros p q.
-    rewrite /own_full_encoded_history_loc.
-    iSplit.
-    - iIntros "[[$$] #?]". iFrame "#".
-    - iIntros "[[$ $] [$ _]]".
-  Qed.
-  Global Instance own_full_encoded_history_as_fractional γ1 γ2 ℓ q enc_abs_hist :
-    AsFractional
-      (own_full_encoded_history_loc γ1 γ2 ℓ q enc_abs_hist)
-      (λ q, own_full_encoded_history_loc γ1 γ2 ℓ q enc_abs_hist)%I q.
-  Proof. split; [done | apply _]. Qed.
+  (* Global Instance own_full_encoded_history_fractional γ ℓ enc_abs_hist : *)
+  (*   Fractional (λ q, own_full_encoded_history_loc γ ℓ q enc_abs_hist). *)
+  (* Proof. apply _. *)
+  (*   intros p q. *)
+  (*   rewrite /own_full_encoded_history_loc. *)
+  (*   iSplit. *)
+  (*   - iIntros "[[$$] #?]". iFrame "#". *)
+  (*   - iIntros "[[$ $] [$ _]]". *)
+  (* Qed. *)
+  (* Global Instance own_full_encoded_history_as_fractional γ ℓ q enc_abs_hist : *)
+  (*   AsFractional *)
+  (*     (own_full_encoded_history_loc γ ℓ q enc_abs_hist) *)
+  (*     (λ q, own_full_encoded_history_loc γ ℓ q enc_abs_hist)%I q. *)
+  (* Proof. split; [done | apply _]. Qed. *)
 
-  Lemma own_full_history_loc_agree γ1 γ2 ℓ q p abs_hist1 abs_hist2 :
-    own_full_history_loc γ1 γ2 ℓ q abs_hist1 -∗
-    own_full_history_loc γ1 γ2 ℓ p abs_hist2 -∗
+  Lemma history_full_map_loc_agree γ ℓ q p abs_hist1 abs_hist2 :
+    history_full_map_loc γ ℓ q abs_hist1 -∗
+    history_full_map_loc γ ℓ p abs_hist2 -∗
     ⌜ abs_hist1 = abs_hist2 ⌝.
   Proof.
-    iIntros "[A _]".
-    iIntros "[B _]".
-    iDestruct (ghost_map_elem_agree with "A B") as %<-%(inj _).
-    done.
+    iIntros "[A _]". iIntros "[B _]".
+    iDestruct (full_entry_agree with "A B") as %<-%(inj _). done.
   Qed.
 
-  Lemma own_full_history_loc_to_frag γ1 γ2 ℓ q abs_hist :
-    own_full_history_loc γ1 γ2 ℓ q abs_hist -∗
-    own_frag_history_loc γ2 ℓ abs_hist.
-  Proof.
-    iIntros "[_ H]". iExists _. iFrame "H".
-    iPureIntro.
-    apply map_eq. intros t.
-    rewrite 3!lookup_fmap.
-    destruct (abs_hist !! t); last done.
-    simpl. rewrite decode_encode. done.
-  Qed.
+  (* Lemma history_full_map_loc_to_frag γ ℓ q abs_hist : *)
+  (*   history_full_map_loc γ ℓ q abs_hist -∗ *)
+  (*   history_frag_entry_unenc γ ℓ abs_hist. *)
+  (* Proof. *)
+  (*   iIntros "[_ H]". iExists _. iFrame "H". *)
+  (*   iPureIntro. *)
+  (*   apply map_eq. intros t. *)
+  (*   rewrite 3!lookup_fmap. *)
+  (*   destruct (abs_hist !! t); last done. *)
+  (*   simpl. rewrite decode_encode. done. *)
+  (* Qed. *)
 
-  Lemma own_frag_history_loc_lookup γ2 ℓ abs_hist t h :
-    abs_hist !! t = Some h →
-    own_frag_history_loc γ2 ℓ abs_hist -∗
-    own_frag_history_loc γ2 ℓ {[ t := h ]}.
-  Proof.
-    iIntros (look).
-    iIntros "(%m & %eq & H)".
-    setoid_rewrite map_eq_iff in eq.
-    specialize (eq t).
-    rewrite 2!lookup_fmap in eq.
-    rewrite look in eq.
-    simpl in eq.
-    rewrite -lookup_fmap in eq.
-    apply lookup_fmap_Some in eq as (e & dec & mLook).
-    iExists ({[ t := e ]}).
-    iDestruct (auth_map_map_frag_lookup_singleton with "H") as "$".
-    { rewrite lookup_singleton. done. }
-    { done. }
-    iPureIntro.
-    rewrite !map_fmap_singleton.
-    congruence.
-  Qed.
+  (* Lemma history_frag_entry_unenc_lookup ℓ abs_hist t h : *)
+  (*   abs_hist !! t = Some h → *)
+  (*   history_frag_entry_unenc ℓ abs_hist -∗ *)
+  (*   history_frag_entry_unenc ℓ {[ t := h ]}. *)
+  (* Proof. *)
+  (*   iIntros (look). *)
+  (*   iIntros "(%m & %eq & H)". *)
+  (*   setoid_rewrite map_eq_iff in eq. *)
+  (*   specialize (eq t). *)
+  (*   rewrite 2!lookup_fmap in eq. *)
+  (*   rewrite look in eq. *)
+  (*   simpl in eq. *)
+  (*   rewrite -lookup_fmap in eq. *)
+  (*   apply lookup_fmap_Some in eq as (e & dec & mLook). *)
+  (*   iExists ({[ t := e ]}). *)
+  (*   iDestruct (auth_map_map_frag_lookup_singleton with "H") as "$". *)
+  (*   { rewrite lookup_singleton. done. } *)
+  (*   { done. } *)
+  (*   iPureIntro. *)
+  (*   rewrite !map_fmap_singleton. *)
+  (*   congruence. *)
+  (* Qed. *)
 
-  Lemma own_full_history_alloc h :
-    ⊢ |==> ∃ γ1 γ2,
-        own_full_history γ1 γ2 h ∗
-        auth_map_map_frag γ2 h ∗
-        [∗ map] k↦v ∈ h, k ↪[γ1] v.
-  Proof.
-    iMod (ghost_map_alloc h) as (new_abs_history_name) "[A B]".
-    iExists _. iFrame "A B".
-    setoid_rewrite <- own_op.
-    iMod (own_alloc _) as "$".
-    { apply auth_both_valid_2; last reflexivity.
-      intros k.
-      rewrite lookup_fmap.
-      case (h !! k); simpl; last done.
-      intros ? k'.
-      apply Some_valid.
-      rewrite lookup_fmap.
-      case (g !! k'); done. }
-    done.
-  Qed.
+  (* Lemma history_full_map_alloc h : *)
+  (*   ⊢ |==> ∃ γ , *)
+  (*       history_full_map γ h ∗ *)
+  (*       auth_map_map_frag h ∗ *)
+  (*       [∗ map] k↦v ∈ h, k ↪[γ] v. *)
+  (* Proof. *)
+  (*   iMod (ghost_map_alloc h) as (new_abs_history_name) "[A B]". *)
+  (*   iExists _. iFrame "A B". *)
+  (*   setoid_rewrite <- own_op. *)
+  (*   iMod (own_alloc _) as "$". *)
+  (*   { apply auth_both_valid_2; last reflexivity. *)
+  (*     intros k. *)
+  (*     rewrite lookup_fmap. *)
+  (*     case (h !! k); simpl; last done. *)
+  (*     intros ? k'. *)
+  (*     apply Some_valid. *)
+  (*     rewrite lookup_fmap. *)
+  (*     case (g !! k'); done. } *)
+  (*   done. *)
+  (* Qed. *)
 
-  Lemma own_full_equiv γ1 γ2 ℓ q abs_hist :
-    own_full_history_loc γ1 γ2 ℓ q abs_hist ⊣⊢
-      own_full_encoded_history_loc γ1 γ2 ℓ q (encode <$> abs_hist).
+  Lemma own_full_equiv γ ℓ q abs_hist :
+    history_full_map_loc γ ℓ q abs_hist ⊣⊢
+      own_full_encoded_history_loc γ ℓ q (encode <$> abs_hist).
   Proof. done. Qed.
 
-  Lemma own_frag_equiv γ ℓ abs_hist :
-    own_frag_encoded_history_loc γ ℓ (encode <$> abs_hist) ⊢
-    own_frag_history_loc γ ℓ abs_hist.
-  Proof.
-    rewrite /own_frag_history_loc /own_frag_encoded_history_loc.
-    iIntros "H".
-    iExists _. iFrame. iPureIntro.
-    apply map_eq. intros t.
-    rewrite !lookup_fmap.
-    destruct (abs_hist !! t); last done.
-    simpl. by rewrite decode_encode.
-  Qed.
+  (* Lemma own_frag_equiv γ ℓ abs_hist : *)
+  (*   history_frag_entry γ ℓ (encode <$> abs_hist) ⊢ *)
+  (*   history_frag_entry_unenc γ ℓ abs_hist. *)
+  (* Proof. *)
+  (*   rewrite /history_frag_entry_unenc /history_frag_entry. *)
+  (*   iIntros "H". *)
+  (*   iExists _. iFrame. iPureIntro. *)
+  (*   apply map_eq. intros t. *)
+  (*   rewrite !lookup_fmap. *)
+  (*   destruct (abs_hist !! t); last done. *)
+  (*   simpl. by rewrite decode_encode. *)
+  (* Qed. *)
 
-  Lemma abs_hist_to_ra_inj hist hist' :
-    abs_hist_to_ra hist' ≡ abs_hist_to_ra hist →
-    hist' = hist.
-  Proof.
-    intros eq.
-    apply: map_eq. intros t.
-    pose proof (eq t) as eq'.
-    rewrite !lookup_fmap in eq'.
-    destruct (hist' !! t) as [h|] eqn:leq, (hist !! t) as [h'|] eqn:leq';
-      try inversion eq'; auto.
-    simpl in eq'.
-    apply Some_equiv_inj in eq'.
-    apply to_agree_inj in eq'.
-    apply encode_inj in eq'.
-    rewrite eq'.
-    done.
-  Qed.
+  (* Lemma abs_hist_to_ra_inj hist hist' : *)
+  (*   abs_hist_to_ra hist' ≡ abs_hist_to_ra hist → *)
+  (*   hist' = hist. *)
+  (* Proof. *)
+  (*   intros eq. *)
+  (*   apply: map_eq. intros t. *)
+  (*   pose proof (eq t) as eq'. *)
+  (*   rewrite !lookup_fmap in eq'. *)
+  (*   destruct (hist' !! t) as [h|] eqn:leq, (hist !! t) as [h'|] eqn:leq'; *)
+  (*     try inversion eq'; auto. *)
+  (*   simpl in eq'. *)
+  (*   apply Some_equiv_inj in eq'. *)
+  (*   apply to_agree_inj in eq'. *)
+  (*   apply encode_inj in eq'. *)
+  (*   rewrite eq'. *)
+  (*   done. *)
+  (* Qed. *)
 
-  Lemma abs_hist_to_ra_agree hist hist' :
-    to_agree <$> hist' ≡ abs_hist_to_ra hist → hist' = encode <$> hist.
-  Proof.
-    intros eq.
-    apply: map_eq. intros t.
-    pose proof (eq t) as eq'.
-    rewrite !lookup_fmap in eq'.
-    rewrite lookup_fmap.
-    destruct (hist' !! t) as [h|] eqn:leq, (hist !! t) as [h'|] eqn:leq';
-      try inversion eq'; auto.
-    simpl in eq'. simpl.
-    apply Some_equiv_inj in eq'.
-    apply to_agree_inj in eq'.
-    f_equiv.
-    apply eq'.
-  Qed.
+  (* Lemma abs_hist_to_ra_agree hist hist' : *)
+  (*   to_agree <$> hist' ≡ abs_hist_to_ra hist → hist' = encode <$> hist. *)
+  (* Proof. *)
+  (*   intros eq. *)
+  (*   apply: map_eq. intros t. *)
+  (*   pose proof (eq t) as eq'. *)
+  (*   rewrite !lookup_fmap in eq'. *)
+  (*   rewrite lookup_fmap. *)
+  (*   destruct (hist' !! t) as [h|] eqn:leq, (hist !! t) as [h'|] eqn:leq'; *)
+  (*     try inversion eq'; auto. *)
+  (*   simpl in eq'. simpl. *)
+  (*   apply Some_equiv_inj in eq'. *)
+  (*   apply to_agree_inj in eq'. *)
+  (*   f_equiv. *)
+  (*   apply eq'. *)
+  (* Qed. *)
 
   (** If you know the full history for a location and own the "all-knowing"
   resource, then those two will agree. *)
-  Lemma own_full_history_agree γ1 γ2 ℓ q hist hists :
-    own_full_history γ1 γ2 hists -∗
-    own_full_history_loc γ1 γ2 ℓ q hist -∗
+  Lemma history_full_map_agree γ ℓ q hist hists :
+    history_full_map γ hists -∗
+    history_full_map_loc γ ℓ q hist -∗
     ⌜hists !! ℓ = Some (encode <$> hist)⌝.
   Proof.
-    iIntros "[A _] [B _]".
-    iApply (ghost_map_lookup with "[$] [$]").
+    iIntros "A [B _]".
+    iApply (full_map_full_entry with "A B").
   Qed.
 
-  Lemma own_frag_history_agree γ1 γ2 ℓ (part_hist : gmap time ST) hists :
-    own_full_history γ1 γ2 hists -∗
-    own_frag_history_loc γ2 ℓ part_hist -∗
-    ⌜∃ hist, hists !! ℓ = Some (hist) ∧
-            (Some <$> part_hist) ⊆ (decode <$> hist)⌝.
-  Proof.
-    rewrite /own_full_history.
-    iIntros "[O A]".
-    iDestruct 1 as (enc) "[%eq K]".
-    iDestruct (own_valid_2 with "A K") as %[incl _]%auth_both_valid_discrete.
-    apply fmap_fmap_to_agree_singleton_included_l in incl.
-    destruct incl as [hist' [look incl]].
-    iPureIntro.
-    exists hist'.
-    split. { apply leibniz_equiv. done. }
-    rewrite -eq. apply map_fmap_mono. done.
-  Qed.
+  (* Lemma own_frag_history_agree γ ℓ (part_hist : gmap time ST) hists : *)
+  (*   history_full_map γ hists -∗ *)
+  (*   history_frag_entry_unenc ℓ part_hist -∗ *)
+  (*   ⌜∃ hist, hists !! ℓ = Some (hist) ∧ *)
+  (*           (Some <$> part_hist) ⊆ (decode <$> hist)⌝. *)
+  (* Proof. *)
+  (*   rewrite /history_full_map. *)
+  (*   iIntros "[O A]". *)
+  (*   iDestruct 1 as (enc) "[%eq K]". *)
+  (*   iDestruct (own_valid_2 with "A K") as %[incl _]%auth_both_valid_discrete. *)
+  (*   apply fmap_fmap_to_agree_singleton_included_l in incl. *)
+  (*   destruct incl as [hist' [look incl]]. *)
+  (*   iPureIntro. *)
+  (*   exists hist'. *)
+  (*   split. { apply leibniz_equiv. done. } *)
+  (*   rewrite -eq. apply map_fmap_mono. done. *)
+  (* Qed. *)
 
-  Lemma own_full_history_frag_singleton_agreee γ1 γ2 ℓ t (s : ST) hists :
-    own_full_history γ1 γ2 hists -∗
-    own_frag_history_loc γ2 ℓ {[ t := s ]} -∗
+  Lemma history_full_map_frag_singleton_agreee γ ℓ t (s : ST) hists :
+    history_full_map γ hists -∗
+    history_frag_entry_unenc γ ℓ t s -∗
     ⌜∃ hist enc,
       hists !! ℓ = Some hist ∧ hist !! t = Some enc ∧ decode enc = Some s⌝.
   Proof.
-    iIntros "H1 H2".
-    iDestruct (own_frag_history_agree with "H1 H2") as %[hist [look H1]].
-    iExists hist. iPureIntro.
-    rewrite map_fmap_singleton in H1.
-    rewrite -> map_subseteq_spec in H1.
-    specialize H1 with t (Some s).
-    epose proof (H1 _) as H2.
-    Unshelve. 2: { rewrite lookup_singleton. done. }
-    apply lookup_fmap_Some in H2.
-    destruct H2 as (enc & eq & lookHist).
-    exists enc.
-    repeat split; done.
+    iIntros "H1 (% & % & H2)".
+    iDestruct (full_map_frag_entry with "H1 H2") as %(mi & EQ & hq).
+    iPureIntro. eexists _, _. split_and!; done.
   Qed.
 
-  Lemma own_full_history_lookup γ1 γ2 abs_hists enc_abs_hist ℓ t s :
-    abs_hists !! ℓ = Some enc_abs_hist →
-    enc_abs_hist !! t = Some s →
-    own_full_history γ1 γ2 abs_hists ==∗
-    own_full_history γ1 γ2 abs_hists ∗
-    own_frag_encoded_history_loc γ2 ℓ {[ t := s ]}.
-  Proof.
-    iIntros (look1 look2).
-    iIntros "[M N]".
-    iMod (auth_map_map_lookup with "N") as "[N hip]"; try done.
-    iFrame.
-    done.
-  Qed.
+  (* Lemma history_full_map_lookup γ abs_hists enc_abs_hist ℓ t s : *)
+  (*   abs_hists !! ℓ = Some enc_abs_hist → *)
+  (*   enc_abs_hist !! t = Some s → *)
+  (*   history_full_map γ abs_hists ==∗ *)
+  (*   history_full_map γ abs_hists ∗ *)
+  (*   history_frag_entry γ ℓ t s. *)
+  (* Proof. *)
+  (*   iIntros (look1 look2). *)
+  (*   iIntros "[M N]". *)
+  (*   iMod (auth_map_map_lookup with "N") as "[N hip]"; try done. *)
+  (*   iFrame. *)
+  (*   done. *)
+  (* Qed. *)
 
-  Lemma own_frag_history_singleton_agreee γ2 ℓ t s1 s2 :
-    own_frag_history_loc γ2 ℓ {[ t := s1 ]} -∗
-    own_frag_history_loc γ2 ℓ {[ t := s2 ]} -∗
+  Lemma own_frag_history_singleton_agreee γ ℓ t s1 s2 :
+    history_frag_entry_unenc γ ℓ t s1 -∗
+    history_frag_entry_unenc γ ℓ t s2 -∗
     ⌜ s1 = s2 ⌝.
   Proof.
-    rewrite /own_frag_history_loc.
-    rewrite !map_fmap_singleton.
-    iDestruct 1 as (enc (e & deq & encEq)%map_fmap_singleton_inv) "K".
-    iDestruct 1 as (enc' (e' & deq' & encEq')%map_fmap_singleton_inv) "K'".
-    rewrite encEq.
-    rewrite encEq'.
-    iDestruct (own_valid_2 with "K K'") as %val%auth_frag_op_valid_1.
-    iPureIntro. move: val.
-    rewrite 2!fmap_fmap_to_agree_singleton.
-    rewrite 2!map_fmap_singleton.
-    rewrite singleton_op.
-    rewrite singleton_valid.
-    rewrite singleton_op.
-    rewrite singleton_valid.
-    intros eq%to_agree_op_inv_L.
-    congruence.
+    iDestruct 1 as (enc deq) "K".
+    iDestruct 1 as (enc' deq') "K'".
+    iDestruct (frag_entry_agree with "K K'") as %<-.
+    iPureIntro. congruence.
   Qed.
 
-  Lemma own_full_history_alloc_frag γ1 γ2 ℓ t encS (s : ST) hists hist :
-    hists !! ℓ = Some hist →
-    hist !! t = Some encS →
-    decode encS = Some s →
-    own_full_history γ1 γ2 hists ==∗
-    own_full_history γ1 γ2 hists ∗ own_frag_history_loc γ2 ℓ {[ t := s ]}.
-  Proof.
-    iIntros (look lookHist decEq) "M".
-    iMod (own_full_history_lookup with "M") as "[M hi]"; try done.
-    iFrame. iModIntro.
-    rewrite /own_frag_history_loc.
-    iExists {[ t := encS ]}.
-    rewrite /own_frag_encoded_history_loc.
-    rewrite !map_fmap_singleton.
-    rewrite decEq.
-    iFrame.
-    done.
-  Qed.
+  (* Lemma history_full_map_alloc_frag γ ℓ t encS (s : ST) hists hist : *)
+  (*   hists !! ℓ = Some hist → *)
+  (*   hist !! t = Some encS → *)
+  (*   decode encS = Some s → *)
+  (*   history_full_map γ hists ==∗ *)
+  (*   history_full_map γ hists ∗ history_frag_entry_unenc γ ℓ {[ t := s ]}. *)
+  (* Proof. *)
+  (*   iIntros (look lookHist decEq) "M". *)
+  (*   iMod (history_full_map_lookup with "M") as "[M hi]"; try done. *)
+  (*   iFrame. iModIntro. *)
+  (*   rewrite /history_frag_entry_unenc. *)
+  (*   iExists {[ t := encS ]}. *)
+  (*   rewrite /history_frag_entry. *)
+  (*   rewrite !map_fmap_singleton. *)
+  (*   rewrite decEq. *)
+  (*   iFrame. *)
+  (*   done. *)
+  (* Qed. *)
 
   (* Insert a new location into an abstract history. *)
-  Lemma own_full_history_history_insert_loc γ1 γ2 abs_hists ℓ enc_abs_hist :
+  Lemma history_full_map_history_insert_loc γ abs_hists ℓ enc_abs_hist :
     abs_hists !! ℓ = None →
-    own_full_history γ1 γ2 abs_hists ==∗
-    own_full_history γ1 γ2 (<[ℓ := enc_abs_hist]>abs_hists) ∗
-    own_full_encoded_history_loc γ1 γ2 ℓ 1 enc_abs_hist.
-    (* own_frag_encoded_history_loc γ2 ℓ enc_abs_hist. *)
+    history_full_map γ abs_hists ==∗
+    history_full_map γ (<[ℓ := enc_abs_hist]>abs_hists) ∗
+    own_full_encoded_history_loc γ ℓ 1 enc_abs_hist.
+    (* history_frag_entry γ ℓ enc_abs_hist. *)
   Proof.
     iIntros (look) "[A B]".
     iMod (ghost_map_insert with "A") as "[$ $]"; first done.
     iMod (auth_map_map_insert_top with "B") as "[$ F]"; first done.
-    rewrite /own_frag_encoded_history_loc.
+    rewrite /history_frag_entry.
     rewrite /auth_map_map_frag.
     rewrite fmap_fmap_to_agree_singleton.
     done.
   Qed.
 
   (* Insert a new message into an abstract history. *)
-  Lemma own_full_encoded_history_insert γ1 γ2 ℓ t enc_abs_hist abs_hists encS :
+  Lemma own_full_encoded_history_insert γ ℓ t enc_abs_hist abs_hists encS :
     enc_abs_hist !! t = None →
-    own_full_history γ1 γ2 abs_hists -∗
-    own_full_encoded_history_loc γ1 γ2 ℓ 1 enc_abs_hist ==∗
+    history_full_map γ abs_hists -∗
+    own_full_encoded_history_loc γ ℓ 1 enc_abs_hist ==∗
     let enc_abs_hist' := <[t := encS]>enc_abs_hist
-    in own_full_history γ1 γ2 (<[ℓ := enc_abs_hist']>abs_hists) ∗
-       own_full_encoded_history_loc γ1 γ2 ℓ 1 enc_abs_hist' ∗
-       own_frag_encoded_history_loc γ2 ℓ {[ t := encS ]}.
+    in history_full_map γ (<[ℓ := enc_abs_hist']>abs_hists) ∗
+       own_full_encoded_history_loc γ ℓ 1 enc_abs_hist' ∗
+       history_frag_entry γ ℓ {[ t := encS ]}.
   Proof.
     iIntros (look) "[M N] [O P]".
     iDestruct (ghost_map_lookup with "M O") as %hips.
@@ -339,20 +318,20 @@ Section abs_history_lemmas.
   Qed.
 
   (* Insert a new message into an abstract history. *)
-  Lemma own_full_history_insert γ1 γ2 ℓ t abs_hist abs_hists (s : ST) :
+  Lemma history_full_map_insert γ ℓ t abs_hist abs_hists (s : ST) :
     abs_hist !! t = None →
-    own_full_history γ1 γ2 abs_hists -∗
-    own_full_history_loc γ1 γ2 ℓ 1 abs_hist ==∗
+    history_full_map γ abs_hists -∗
+    history_full_map_loc γ ℓ 1 abs_hist ==∗
     let abs_hist' := <[t := s]>abs_hist
-    in own_full_history γ1 γ2 (<[ℓ := encode <$> abs_hist']>abs_hists) ∗
-       own_full_history_loc γ1 γ2 ℓ 1 abs_hist' ∗
-       own_frag_history_loc γ2 ℓ {[ t := s ]}.
+    in history_full_map γ (<[ℓ := encode <$> abs_hist']>abs_hists) ∗
+       history_full_map_loc γ ℓ 1 abs_hist' ∗
+       history_frag_entry_unenc γ ℓ {[ t := s ]}.
   Proof.
     iIntros (look) "??".
     iMod (own_full_encoded_history_insert with "[$] [$]") as "(H1 & H2 & H3)".
     { rewrite lookup_fmap. apply fmap_None. done. }
     iModIntro.
-    rewrite /own_full_history_loc /own_frag_history_loc fmap_insert.
+    rewrite /history_full_map_loc /history_frag_entry_unenc fmap_insert.
     iFrame "H1 H2".
     iExists _. iFrame.
     rewrite !map_fmap_singleton. by rewrite decode_encode.
